<?xml version="1.0"?>


<!DOCTYPE rdf:RDF [
    <!ENTITY owl "http://www.w3.org/2002/07/owl#" >
    <!ENTITY dc "http://purl.org/dc/elements/1.1/" >
    <!ENTITY xsd "http://www.w3.org/2001/XMLSchema#" >
    <!ENTITY rk "http://cogbotserver/onto/robokind#" >
    <!ENTITY grddl "http://www.w3.org/2003/g/data-view#" >
    <!ENTITY rdfs "http://www.w3.org/2000/01/rdf-schema#" >
    <!ENTITY rdf "http://www.w3.org/1999/02/22-rdf-syntax-ns#" >
]>


<rdf:RDF xmlns="http://cogbotserver/onto/robokind#"
     xml:base="http://cogbotserver/onto/robokind#"
     xmlns:dc="http://purl.org/dc/elements/1.1/"
     xmlns:rdfs="http://www.w3.org/2000/01/rdf-schema#"
     xmlns:rk="http://cogbotserver/onto/robokind#"
     xmlns:owl="http://www.w3.org/2002/07/owl#"
     xmlns:xsd="http://www.w3.org/2001/XMLSchema#"
     xmlns:rdf="http://www.w3.org/1999/02/22-rdf-syntax-ns#"
     xmlns:grddl="http://www.w3.org/2003/g/data-view#">
    <owl:Ontology rdf:about="http://cogbotserver/onto/robokind">
        <owl:versionInfo>$Date: 2012/11/15 10:54:12 $</owl:versionInfo>
        <rdfs:comment>
  This ontology partially describes the built-in classes and
  properties that together form the basis of the RDF/XML syntax of OWL 2.
  The content of this ontology is based on Tables 6.1 and 6.2
  in Section 6.4 of the OWL 2 RDF-Based Semantics specification,
  available at http://www.w3.org/TR/owl2-rdf-based-semantics/.
  Please note that those tables do not include the different annotations
  (labels, comments and rdfs:isDefinedBy links) used in this file.
  Also note that the descriptions provided in this ontology do not
  provide a complete and correct formal description of either the syntax
  or the semantics of the introduced terms (please see the OWL 2
  recommendations for the complete and normative specifications).
  Furthermore, the information provided by this ontology may be
  misleading if not used with care. This ontology SHOULD NOT be imported
  into OWL ontologies. Importing this file into an OWL 2 DL ontology
  will cause it to become an OWL 2 Full ontology and may have other,
  unexpected, consequences.
   </rdfs:comment>
        <dc:title>Cogbot Schema vocabulary</dc:title>
        <owl:versionIRI rdf:resource="http://cogbotserver/onto/robokind"/>
        <grddl:namespaceTransformation rdf:resource="http://dev.w3.org/cvsweb/2009/owl-grddl/owx2rdf.xsl"/>
        <owl:imports rdf:resource="http://www.w3.org/2000/01/rdf-schema"/>
        <owl:imports rdf:resource="http://www.w3.org/2002/07/owl"/>
        <rdfs:isDefinedBy rdf:resource="http://www.w3.org/TR/owl2-mapping-to-rdf/"/>
        <rdfs:isDefinedBy rdf:resource="http://www.w3.org/TR/owl2-rdf-based-semantics/"/>
        <rdfs:seeAlso rdf:resource="http://www.w3.org/TR/owl2-rdf-based-semantics/#table-axiomatic-classes"/>
        <rdfs:seeAlso rdf:resource="http://www.w3.org/TR/owl2-rdf-based-semantics/#table-axiomatic-properties"/>
        <rdfs:isDefinedBy rdf:resource="http://www.w3.org/TR/owl2-syntax/"/>
    </owl:Ontology>
    


    <!-- 
    ///////////////////////////////////////////////////////////////////////////////////////
    //
    // Annotation properties
    //
    ///////////////////////////////////////////////////////////////////////////////////////
     -->

    


    <!-- 
    ///////////////////////////////////////////////////////////////////////////////////////
    //
    // Datatypes
    //
    ///////////////////////////////////////////////////////////////////////////////////////
     -->

    


    <!-- 
    ///////////////////////////////////////////////////////////////////////////////////////
    //
    // Object Properties
    //
    ///////////////////////////////////////////////////////////////////////////////////////
     -->

    


    <!-- http://cogbotserver/onto/robokind#prologMappingType -->

    <owl:ObjectProperty rdf:about="&rk;prologMappingType">
        <rdfs:domain rdf:resource="&rk;PrologInRDFPredicate"/>
        <rdfs:range rdf:resource="&rk;PrologPredicateMappingType"/>
    </owl:ObjectProperty>
    


    <!-- 
    ///////////////////////////////////////////////////////////////////////////////////////
    //
    // Data properties
    //
    ///////////////////////////////////////////////////////////////////////////////////////
     -->

    


    <!-- http://cogbotserver/onto/robokind#prologArity -->

    <owl:DatatypeProperty rdf:about="&rk;prologArity">
        <rdf:type rdf:resource="&owl;FunctionalProperty"/>
        <rdfs:comment>Expected arity of Prolog Predicate</rdfs:comment>
        <rdfs:domain rdf:resource="&rk;PrologInRDFPredicate"/>
        <rdfs:range rdf:resource="&xsd;nonNegativeInteger"/>
    </owl:DatatypeProperty>
    


    <!-- http://cogbotserver/onto/robokind#prologAxiomValueArg -->

    <owl:DatatypeProperty rdf:about="&rk;prologAxiomValueArg">
        <rdfs:comment>If the Assertion is an Instance.. then Axiom created has some truth value found in this argument of the original</rdfs:comment>
        <rdfs:domain rdf:resource="&rk;PrologInRDFPredicate"/>
        <rdfs:range rdf:resource="&xsd;nonNegativeInteger"/>
    </owl:DatatypeProperty>
    


    <!-- http://cogbotserver/onto/robokind#prologInstanceArg -->

    <owl:DatatypeProperty rdf:about="&rk;prologInstanceArg">
        <rdf:type rdf:resource="&owl;FunctionalProperty"/>
        <rdfs:comment>The subject is in this arg</rdfs:comment>
        <rdfs:range rdf:resource="&xsd;nonNegativeInteger"/>
        <rdfs:domain rdf:resource="&owl;ObjectProperty"/>
    </owl:DatatypeProperty>
    


    <!-- 
    ///////////////////////////////////////////////////////////////////////////////////////
    //
    // Classes
    //
    ///////////////////////////////////////////////////////////////////////////////////////
     -->

    


    <!-- http://cogbotserver/onto/robokind#PrologArgPredicate -->

    <owl:Class rdf:about="&rk;PrologArgPredicate">
        <rdfs:subClassOf rdf:resource="&owl;FunctionalProperty"/>
        <rdfs:subClassOf rdf:resource="&owl;ObjectProperty"/>
    </owl:Class>
    


    <!-- http://cogbotserver/onto/robokind#PrologInRDFPredicate -->

    <owl:Class rdf:about="&rk;PrologInRDFPredicate">
        <rdfs:subClassOf rdf:resource="&owl;ObjectProperty"/>
    </owl:Class>
    


    <!-- http://cogbotserver/onto/robokind#PrologPredicateMappingType -->

    <owl:Class rdf:about="&rk;PrologPredicateMappingType"/>
    


    <!-- http://www.w3.org/1999/02/22-rdf-syntax-ns#Property -->

    <owl:Class rdf:about="&rdf;Property"/>
    


    <!-- http://www.w3.org/2002/07/owl#FunctionalProperty -->

    <owl:Class rdf:about="&owl;FunctionalProperty"/>
    


    <!-- http://www.w3.org/2002/07/owl#ObjectProperty -->

    <owl:Class rdf:about="&owl;ObjectProperty">
        <rdfs:label>ObjectProperty</rdfs:label>
        <rdfs:subClassOf rdf:resource="&rdf;Property"/>
        <rdfs:comment>The class of object properties.</rdfs:comment>
        <rdfs:isDefinedBy rdf:resource="http://www.w3.org/2002/07/owl#"/>
    </owl:Class>
    


    <!-- 
    ///////////////////////////////////////////////////////////////////////////////////////
    //
    // Individuals
    //
    ///////////////////////////////////////////////////////////////////////////////////////
     -->

    


    <!-- http://cogbotserver/onto/robokind#DirectOneToOneMapping -->

    <owl:NamedIndividual rdf:about="&rk;DirectOneToOneMapping">
        <rdf:type rdf:resource="&rk;PrologPredicateMappingType"/>
        <rdfs:comment>The Assertion Predicate is mapped literally .. this means the prologInstanceArg must be 1 with a URI in first arg</rdfs:comment>
    </owl:NamedIndividual>
    


    <!-- http://cogbotserver/onto/robokind#InstanceOnArg -->

    <owl:NamedIndividual rdf:about="&rk;InstanceOnArg">
        <rdf:type rdf:resource="&rk;PrologPredicateMappingType"/>
        <rdfs:comment>States that if the predicate is instanced On an Argument the Arg becomes the &quot;Subject&quot; this can still be used on Arity 2 Predicates</rdfs:comment>
    </owl:NamedIndividual>
    


    <!-- http://cogbotserver/onto/robokind#MapEachArgToProperty -->

    <owl:NamedIndividual rdf:about="&rk;MapEachArgToProperty">
        <rdf:type rdf:resource="&rk;PrologPredicateMappingType"/>
        <rdfs:comment>The assertion is Instanced as a PrologAssertion and each argument is the Object in pred_arg1(assertionInstance,arg1Value) </rdfs:comment>
    </owl:NamedIndividual>



    <!-- http://cogbotserver/onto/robokind#PrologOnlyPredicate -->

    <owl:NamedIndividual rdf:about="&rk;PrologOnlyPredicate">
        <rdf:type rdf:resource="&rk;PrologPredicateMappingType"/>
        <rdfs:comment>Prolog only predicates are predicates that are intended to not be represented in RDF</rdfs:comment>
    </owl:NamedIndividual>



    <!-- http://cogbotserver/onto/robokind#MappingTODO -->

    <owl:NamedIndividual rdf:about="&rk;MappingTODO">
        <rdf:type rdf:resource="&rk;PrologPredicateMappingType"/>
        <rdfs:comment>This means that we cannot yet map this predicate</rdfs:comment>
    </owl:NamedIndividual>
    


    <!-- 
    ///////////////////////////////////////////////////////////////////////////////////////
    //
    // General axioms
    //
    ///////////////////////////////////////////////////////////////////////////////////////
     -->

    <rdf:Description>
        <rdf:type rdf:resource="&owl;AllDifferent"/>
        <owl:distinctMembers rdf:parseType="Collection">
            <rdf:Description rdf:about="&rk;DirectOneToOneMapping"/>
            <rdf:Description rdf:about="&rk;MapEachArgToProperty"/>
            <rdf:Description rdf:about="&rk;PrologOnlyPredicate"/>
        </owl:distinctMembers>
    </rdf:Description>
</rdf:RDF>



<!-- Generated by the OWL API (version 3.3.1957) http://owlapi.sourceforge.net -->

